state/Examples.Hello.fst
@@ -9,20 +9,20 @@ open LabeledRefs
 open Witnessable
 
 let hello0 ()
-  : SST (ref int)
+  : LR (ref int)
     (requires (fun h0 -> True))
     (ensures (fun h0 _ h1 -> True)) =
     sst_alloc_shareable #SNat 1
 
 let hello ()
-  : SST unit
+  : LR unit
     (requires (fun h0 -> True))
     (ensures (fun h0 () h1 -> True)) =
     let ref_ll = sst_alloc_shareable #SNat 1 in 
     ()
 
 let hello_read_write ()
-  : SST unit
+  : LR unit
     (requires (fun h0 -> False))
     (ensures (fun h0 () h1 -> True)) =
     let ref = sst_alloc_shareable #SNat 1 in 
